FromAxioms/Analysis.lean
@@ -21,3 +21,4 @@ import FromAxioms.Analysis.Complex
 import FromAxioms.Analysis.InnerProduct
 import FromAxioms.Analysis.InnerSpace
 import FromAxioms.Analysis.DirichletChar
+import FromAxioms.Analysis.HahnBanach
